#+TITLE:Some solutions to problems from the 2025 IMO
#+DESCRIPTION:Directory
#+HTML_HEAD: <link rel="stylesheet" type="text/css" href="https://gongzhitaao.org/orgcss/org.css"/>
#+HTML_HEAD: <style> body {font-size:15px;} </style>

/Originally posted:/

-------------

* Introduction

Inspired by Prof. Timothy Gowers' YouTube videos, I recently attempted to solve some IMO problems!

* IMO 2025

** Problem 1

Here is the first problem:


#+ATTR_HTML: :width 750px
[[./assets/imo_q1.png]]

and here is my solution:

*Claim 2.1.* Any cover $C = \{L_1, \dots, L_n\}$ of the ``integer triangle" of $(a, b) \in \mathbb{Z}^2_{> 0}$ with $a + b \leq n + 1$ by $n$ lines must include a non-sunny line along one of its edges.

/Proof./ Suppose not. Label the edges $E_1, E_2, E_3$. Each $E_j$ has $n$ points, and they share corners. If some $L_k \in C$ passes through two points common to the same $E_j$, then $L_k = E_j$. Thus,
each of the $n$ points of fixed $E_j$ are contained in unique $L_k$. In the $E_j$ combined, there are $3n - 3$ points, so for $n > 3$, we have $3n - 3 > 2n$, which means that by the
Pigeonhole principle, some $L_k$ must contain at least three distinct points of the combined $E_j$, and they must be from distinct $E_j$ (as we explained). But such points cannot be colinear, so this is a contradiction. $\blacksquare$

Thus, if $C$ is a covering for the integer triangle for some $n > 3$, with $k$ sunny lines, we can write it as $C = \{L_1, \dots, L_{n - 1}, E_j\}$ for some $E_j$. This $E_j$ is not sunny.
Removing this $E_j$ and the corresponding points, we get a cover $\{L_1, \dots, L_{n - 1}\}$ by $n - 1$ lines of the integer
triangle for the case of $n - 1$, again with $k$ sunny lines. Thus, we inductively reduce to the case of $n = 3$ without changing $k$. In this case, we can easily write down coverings with $0$, $1$, or $3$ sunny lines:

#+ATTR_HTML: :width 600px
[[./assets/triangles.png]]

and it follows that since we can reduce to these cases inductively with $k$ invariant, these are the only possibilities for $k$, for any $n \geq 3$. Of course, we can /produce/ such covering for $k = 0, 1, 3$ for
any $n$ as well, by simply adding non-sunny lines to the images above. This completes the proof. $\blacksquare$

** Problem 4

Here is the fourth problem:

#+ATTR_HTML: :width 750px
[[./assets/imo_q4.png]]

and here is my solution:

Call a sequence which satisfies the necessary criteria /valid/.

*Claim 3.1.* A sequence of $a_j$ is valid if and only if $a_1 = 6 \cdot 12^k \cdot q$ for some $k \geq 0$ and odd $q$ which is not divisible by $5$.

The action of mapping some $n \in \mathbb{N}$ to the sum of its largest three proper divisors is exactly

\begin{equation}
\label{eq:trans}
n \mapsto \left( \frac{1}{m_1} + \frac{1}{m_2} + \frac{1}{m_3} \right) n = \left( \frac{m_2 m_3 + m_1 m_3 + m_1 m_2}{m_1 m_2 m_3} \right) n
\end{equation}

where $m_1, m_2, m_3$ are its smallest three divisors (greater than $1$). Note that this map is non-decreasing in only three situations, in particular, $(m_1, m_2, m_3) = (2, 3, 4)$
gives $n \mapsto \frac{13 n}{12}$, $(m_1, m_2, m_3) = (2, 3, 5)$ gives $n \mapsto \frac{31 n}{30}$, and $(m_1, m_2, m_3) = (2, 3, 6)$ gives
$n \mapsto n$. The greatest-coefficient strictly decreasing mapping is given by $(m_1, m_2, m_3) = (2, 3, 7)$, where $n \mapsto \frac{41 n}{42}$. We can characterize a valid
sequence of $a_j$ by an iterated sequence of these maps. In particular, note that if $a_1 = 6 \cdot 12^k \cdot q$, by iterating the map of Eq. \eqref{eq:trans}, we send $6 \cdot 12^k \cdot q$ to
$6 \cdot 13^k \cdot q$ via the map with $(m_1, m_2, m_3) = (2, 3, 4)$. Then via $(m_1, m_2, m_3) = (2, 3, 6)$, the sequence stabilizes. This proves one direction of Claim 1.

Any valid sequence must contain an infinite number of the three non-decreasing mappings, otherwise we would eventually reach a number which does not have at three distinct proper divisors.
This means an infinite number of elements in the sequence must be divisible by $2 \cdot 3 = 6$.


*Claim 3.2.* The map of Eq. \eqref{eq:trans} sends odd $n$ to odd $n$.

/Proof./ In this case, any valid mapping will be for $(m_1, m_2, m_3)$ none of which are even (as $2$ does not divide $n$). Thus $m_2 m_3 + m_1 m_3 + m_1 m_2$ is odd. $\blacksquare$

An immediate corollary of this fact is that in a valid sequence, every element must be even. If $a_N$ were odd for some $N$, then all $a_j$ for $j \geq N$ would be odd, hence not divisible by $6$.
It follows that any mapping going from $a_{j - 1}$ to $a_j$ in a valid sequence is of the form $(m_1, m_2, m_3) = (2, a, b)$. From here, suppose we have a mapping in a valid sequence where both $a$ and
$b$ are odd. Then in particular, $4$ does not divide $a_{j - 1}$ and $2a + 2b + ab$ is odd, while $2ab$ is even. Hence, $a_{j - 1}$ is mapped to something odd, which can't be true for a valid sequence.
Thus, we can always assume that a mapping in a valid sequence is of the form $(2, 4, a)$ or $(2, a, 2a)$, corresponding to mappings

\begin{equation}
\label{eq:trans2}
    n \mapsto \left( \frac{3a + 4}{4a} \right) n \ \ \ \ \text{or} \ \ \ \ n \mapsto \left( \frac{3 + a}{2a} \right) n
\end{equation}

where $a$ is the smallest (greater than $1$) divisor of $a_{j - 1}$ not equal to $2$ or $4$. Note that if $n$ is not divisible by $3$, then mapping under the transformations of
Eq. \eqref{eq:trans2} yields something also indivisible by $3$. Hence, for some logic as earlier (requiring an infitude of elements divisible by $6$), each element of a valid sequence
must be divisible by $3$. Therefore, it must be the case that $a = 3$, and we have two mappings which are admissible in a valid sequence: $(m_1, m_2, m_3) = (2, 3, 4)$ and $(2, 3, 6)$.
\newline

It follows that $a_1$ must be a number whose lowest (greater than $1$) divisors are either $(2, 3, 4)$ or $(2, 3, 6)$. In the latter case, $4$ and $5$ do not divide $a_1$, so $a_1 = 6 \cdot q$ with
$q$ odd indivisible by $5$. In the former case, $a_1 = 12^k \cdot h$ where $h$ is indivisible by $12$. Iterating the $(2, 3, 4)$ -map yields $h$, so the only choice from here is to map under the $(2, 3, 6)$ -map,
meaning $(2, 3, 6)$ are the lowest divisors of $h$, so from the other case, $h = 6 \cdot q$, and we are done. $\blacksquare$

** Problem 3

Here is the third problem:

#+ATTR_HTML: :width 750px
[[./assets/imo_q3.png]]

and here is my solution:

The first thing to notice is that because $f(a) \ | \ b^a - f(b)^{f(a)}$ for all $a$ and $b$, we have $f(a) \ | \ a^a$ for all $a$. In particular, the prime
factors of $f(a)$ are all prime factors of $a$, and if $a = p^n$, a prime power, then $f(a) = p^{N}$ with $0 \leq N \leq n a$. Suppose $p$ is a prime factor of $a > 1$, and
suppose $f(p) = 1$. Then we have $f(a) \ | \ p^{a} - 1$.
However, note that $p$ \emph{does not} divide $p^{a} - 1$, as it would then divide $1$, so it follows that $p$ cannot be a prime factor of $f(a)$. In other words:

*Fact 4.1.* If $p$ is a prime factor of $a$, and $f(p) = 1$, then $p$ is not a prime factor of $f(a)$.

Note that from Euler's theorem, for any $z$ coprime to prime $p$, we have

\begin{equation}
p^n \ | \ z^{\varphi(p^{n})} - 1 = z^{p^n - p^{n - 1}} - 1 \Longrightarrow p^n \ | \ z^{p^n} - z^{p^{n - 1}}
\end{equation}
In fact, the last expression holds for all $z$, as $n \leq 2^{n - 1} \leq p^{n - 1}$ for $n \geq 1$, so if $z = y p$, $p$ divides the right-hand side. Thus,
by induction (and a telescoping sum), $p \ | \ z^{p^n} - z$. In particular, $p \ | \ b^{p^n} - b$ and $p \ | \ f(b)^{p^n} - f(b)$ for any $n$ and $b$. Suppose $f(p) \neq 1$,
then $p \ | \ f(p)$, and because $f(p) \ | \ b^p - f(b)^{f(p)}$, we have $p \ | \ b^{p} - f(b)^{p^M}$ where $p^M = f(p)$. By choosing $n$ appropriately, we arrive at:

*Fact 4.2.* If $f(p) \neq 1$ for some prime $p$, then $p \ | \ f(b) - b$ for all $b$.

*Corollary 4.1.* If $f(a) = 1$, then $f(p) = 1$ for any prime factor $p$ of $a$, as if $f(p) \neq 1$, we would have $p \ | \ a - 1$, which can't be. If $p$ is a prime factor
of $a$ and $f(p) \neq 1$, then $p \ | \ f(a)$ ($p$ is a prime factor of $f(a)$). Combining with Fact 1: a prime factor $p$ of $a$ is a prime factor of $f(a)$ if and only if $f(p) \neq 1$.

*Claim 4.1.* There exist arbitrarily large primes $p$ such that $3$ does not divide $p - 1$.

/Proof./ From Dirichlet's theorem on arithmetic progression, there are an infinite number of primes of the form $p = 3n + 2$. Of course, $p - 1 = 3n + 1$ is not divisible by $3$, for any $n$. $\blacksquare$

Now, $f$ is chosen such that there is some $b$ with $f(b) - b \neq 0$. Then any of the primes $p$ which are not prime factors of $f(b) - b$ will satisfy $f(p) = 1$. By Claim 1, we can
choose $p$ large enough that it doesn't divide $f(b) - b$, \emph{and} such that $3$ does not divide $p - 1$. Note that if $f(p) = 1$ for some prime, then for any other prime $q$ with
$f(q) \neq 1$, we have $q \ | \ p^q - 1$, and since $q \ | \ p^q - p$ as well (from Euler's theorem), $q \ | \ p - 1$. Therefore, we must have $f(3) = 1$, by our choice of $p$.

So, it follows that if $f(p) \neq 1$ for some prime $p$, then $p \ | \ 2$ (Fact 4.2 with $b = 3$), so we must have $p = 2$. In particular, $f = 1$ on all primes except $2$. It then follows
that $f(2^k a) = 2^N$ for some $N$, for every $2^k a$, by Corollary 4.1.

From here, we must have $f(2^k a) = 2^N$ dividing $3^{2^k a} - 1$ for all $2^k a$, where $a$ is odd. Note that
\begin{equation}
    3^{2^k a} - 1 = (3^{2^{k - 1} a} - 1)(3^{2^{k - 1} a} + 1) = (9^{a} - 1)(3^{2a} + 1) \cdots (3^{2^{k - 2} a} + 1) (3^{2^{k - 1} a} + 1)
\end{equation}

Note that $3^{2^j a} + 1 = 2 \ \text{mod} \ 4$, so each of these factors contributes a single $2$ in the prime factorization. In addition,
$9^a - 1 = (2^3 + 1)^a - 1 = 2^3 o$, where $o$ is odd (remember $a$ is odd), so this term contributes three twos. Thus, we have a total of $k + 2$ twos in the prime factorization.
Thus, $N \leq k + 2$. In particular, $f(a) \leq 4 a$ for all $a$. Thus, $c \leq 4$.

To prove that $4$ is optimal, so $c = 4$, we try to produce bonza $f$ such that $f(4) = 16$. Suppose we let $f(2^k a) = 1$ when $k = 0$, $2$ when $k = 1$, and $2^{k + 2}$ when $k \geq 2$.
We need to show that $f(2^k a) \ | \ (2^j b)^{2^k a} - f(2^j b)^{f(2^k a)}$. There is nothing to prove when $j = 0$ or $k = 0$. If $k = 1$ and $j \geq 1$, the claim holds. If $k = 2$,
we have $f(2^k a) = 2^{k + 2}$. We also have $2^{2^k a}$ dividing the right-hand side. Note that $k + 2 \leq 2^k a$ for $k \geq 2$, so we have proved that $f$ is bonza and saturates the bound. $\blacksquare$

* IMO 2024

** Problem 1

Here is my solution:

My claim is that the only possible $\alpha$ which work are even integers. Obviously, even integers /do/ work, because if $\alpha = 2m$, then

\begin{equation}
\lfloor 2m \rfloor + \cdots + \lfloor 2mn \rfloor = 2m (1 + \cdots + n) = \frac{ 2m n (n + 1)}{2} = m n (n + 1)
\end{equation}

for any $n \in \mathbb{N}$. From here, suppose $\alpha = \frac{p}{q}$, a non-integer rational number where $p$ and $q$ are coprime. Let $K = \lfloor \frac{q}{p} \rfloor$.
Of course, the function $f(k) = \lfloor k \alpha \rfloor$ is constant on values of $k \in \{ n K + 1, \dots, nK + K\}$: it is equal to 
